update

theory/Sound_Communication_A.thy
@@ -1211,23 +1211,135 @@ proof -
 
 qed
 
+
+
+
+inductive narrow_step :: "trace_pool * cmmn_set \<Rightarrow> control_path \<Rightarrow> trace_pool * cmmn_set \<Rightarrow> control_path \<Rightarrow> bool" where
+  refl: "
+    E \<pi> \<noteq> None \<Longrightarrow>
+    narrow_step (E, H) \<pi> (E, H) \<pi>" |
+  step: "
+    concur_step (E, H) (Em, Hm) \<Longrightarrow>
+    leaf E \<pi> \<Longrightarrow>
+    Em (\<pi> @ [l]) \<noteq> None \<Longrightarrow>
+    narrow_step (Em, Hm) (\<pi> @ [l]) (E', H') \<pi>' \<Longrightarrow>
+    narrow_step (E, H) \<pi> (E', H') \<pi>'
+  "
+
 lemma static_traversable_pool_implies_static_traceabl_generalized:
   assumes
-    H1: "\<E>' \<pi> = Some (\<langle>e;\<rho>;\<kappa>\<rangle>)" and
-    H2: "\<pi> @ \<pi>Suff = \<pi>'" and
+    H1: "\<E> \<pi> = Some (\<langle>e;\<rho>;\<kappa>\<rangle>)" and
+    H2: "narrow_step (\<E>, H) \<pi> (\<E>', H') \<pi>'" and
     H3: "\<E>' \<pi>' = Some (\<langle>Let x b e\<^sub>n;\<rho>';\<kappa>'\<rangle>)" and
     H4: "(V, C) \<Turnstile>\<^sub>\<E> \<E>'" and
     H5: "static_traversable_pool V F \<E>'" and
     H6: "isEnd (NLet x)"
 
+
   shows "
-    \<exists> path . 
+    \<exists> \<pi>Suff path .
+      \<pi> @ \<pi>Suff = \<pi>' \<and> 
       paths_correspond \<pi>Suff path \<and>
       static_traceable V F (top_label e) isEnd path"
+
 sorry
 
+lemma star_concur_step_implies_narrow_step: 
+  assumes 
+    H1: "star concur_step EH EH'" and
+    H2: "EH = (E, H) \<and> EH' = (E', H')" and
+    H3: "leaf E \<pi>" and
+    H4: "E' \<pi>' \<noteq> None" and
+    H5: "prefix \<pi> \<pi>'"
+
+  shows "narrow_step EH \<pi> EH' \<pi>'"
+
+proof -
+
+  have H6: "
+      \<forall> E H \<pi> .
+      EH = (E, H) \<longrightarrow> EH' = (E', H') \<longrightarrow> 
+      leaf E \<pi> \<longrightarrow> E' \<pi>' \<noteq> None \<longrightarrow> prefix \<pi> \<pi>' \<longrightarrow>
+      narrow_step EH \<pi> EH' \<pi>'"
+  using H1
+  proof induct
+    case (refl x)
+    {
+      fix E H \<pi>
+      assume
+        L2H1: "x = (E, H)" and 
+        L2H2: "x = (E', H')" and 
+        L2H3: "leaf E \<pi>" and
+        L2H4: "E' \<pi>' \<noteq> None" and 
+        L2H5: "prefix \<pi> \<pi>'"
+
+      have L2H6: "\<pi> = \<pi>'" by (metis L2H1 L2H2 L2H3 L2H4 L2H5 leaf.simps Pair_inject prefix_order.dual_order.not_eq_order_implies_strict)
+
+      have "narrow_step x \<pi> x \<pi>'"
+        by (simp add: L2H2 L2H4 L2H6 narrow_step.refl)
+    }
+    then show ?case by blast
+  next
+    case (step x y z)
+    {
+      fix E H \<pi>
+      assume
+        L2H1: "x = (E, H)" and 
+        L2H2: "z = (E', H')" and 
+        L2H3: "leaf E \<pi>" and
+        L2H4: "E' \<pi>' \<noteq> None" and 
+        L2H5: "prefix \<pi> \<pi>'"
+
+      obtain Em Hm where
+        L2H6: "y = (Em, Hm)"
+        by (meson surj_pair)
+
+      have L2H7: "concur_step (E, H) (Em, Hm)"
+        using L2H1 L2H6 step.hyps(1) by auto
+
+      have L2H8: "star concur_step (Em, Hm) (E', H')"
+        using L2H2 L2H6 step.hyps(2) by auto
 
 
+      have L2H9: "\<exists> l . leaf Em (\<pi> @ [l]) \<and> prefix (\<pi> @ [l]) \<pi>'"
+      using L2H7
+      proof cases
+        case (Seq_Step_Down pi x env xk ek envk k v)
+        then show ?thesis sorry
+      next
+        case (Seq_Step pi x b e env k v)
+        then show ?thesis sorry
+      next
+        case (Seq_Step_Up pi x b e env k e' env')
+        then show ?thesis sorry
+      next
+        case (Let_Chan pi x e env k)
+        then show ?thesis sorry
+      next
+        case (Let_Spawn pi x ec e env k)
+        then show ?thesis sorry
+      next
+        case (Let_Sync pis xs xse es envs ks xsc xm envse pir xr xre er envr kr xrc envre c vm)
+        then show ?thesis sorry
+      qed
+    
+      obtain l where L2H10: "leaf Em (\<pi> @ [l]) \<and> prefix (\<pi> @ [l]) \<pi>'" using L2H9 by blast
+
+      have "L2H11": "narrow_step (Em, Hm) (\<pi> @ [l]) (E', H') \<pi>'"
+        using L2H10 L2H2 L2H4 L2H6 L2H9 step.hyps(3) by blast
+
+      have L2H12: "Em (\<pi> @ [l]) \<noteq> None" using leaf.simps L2H10 by blast
+
+      have L2H13: "narrow_step (E, H) \<pi> (E', H') \<pi>'" using L2H11 L2H12 L2H3 L2H7 narrow_step.step by auto
+
+      have "narrow_step x \<pi> z \<pi>'" by (simp add: L2H1 L2H13 L2H2)
+    }
+
+    then show ?case by blast
+  qed
+
+  show ?thesis using H2 H3 H4 H5 H6 by blast
+qed
 
 lemma static_traversable_pool_implies_static_traceable:
   assumes
@@ -1245,11 +1357,12 @@ proof -
   
   have H6: "(V, C) \<Turnstile>\<^sub>\<E> \<E>'" using H2 H3 static_eval_preserved_under_concur_step_star static_eval_to_pool by blast
 
-  have H7: "leaf [[] \<mapsto> \<langle>e;Map.empty;[]\<rangle>] []" using leaf.simps by simp
+  have H7: "[[] \<mapsto> \<langle>e;Map.empty;[]\<rangle>] [] = Some (\<langle>e;Map.empty;[]\<rangle>)" using leaf.simps by simp
 
-  have H8: "\<E>' [] = Some (\<langle>e;Map.empty;[]\<rangle>)" using H2 mapping_preserved_star by auto
 
-  have H9: "[] @ \<pi>' = \<pi>'" by blast
+  have H8: "leaf [[] \<mapsto> \<langle>e;Map.empty;[]\<rangle>] [] " using leaf.simps by simp
+
+  have H9: "narrow_step ([[] \<mapsto> \<langle>e;Map.empty;[]\<rangle>], {}) [] (\<E>', H') \<pi>'" using star_concur_step_implies_narrow_step H1 H2 H8 by blast
 
   show "
     \<exists> path . 
@@ -1257,7 +1370,8 @@ proof -
       static_traceable V F (top_label e) isEnd path"
   using 
     static_traversable_pool_implies_static_traceabl_generalized
-        H1 H2 H3 H4 H5 H6 H7 H8 H9 by blast
+        H1 H2 H3 H4 H5 H6 H7 H8 H9 by (metis append.left_neutral)
+
 qed
 
 
